theories/eris/tutorial/quicksort.v
@@ -1,6 +1,4 @@
-(* We prove functional correctness of randomised quicksort. Since this is a
-   unary property, we work in the UB logic, which has the appropriate adequacy
-   theorem. *)
+(* We prove functional correctness of randomised quicksort. *)
 
 From stdpp Require Import sorting.
 From clutch.common Require Import inject.
@@ -10,16 +8,7 @@ Set Default Proof Using "Type*".
 
 Section quicksort.
 
-  Import list.
-
   Context `{!erisGS Σ}.
-
-  Definition list_remove_nth_unsafe : val :=
-    λ:"l" "n",
-    match: list_remove_nth "l" "n" with
-    | NONE => #()
-    | SOME "v" => "v"
-    end.
 
   Definition partition : expr :=
     let: "negb" := λ:"b", if: "b" then #false else #true in
@@ -31,30 +20,13 @@ Section quicksort.
   Definition qs : val :=
     rec: "qs" "l" :=
       let: "n" := list_length "l" in
-      if: "n" < #1 then "l" else
+      if: "n" ≤ #1 then "l" else
         let: "ip" := rand ("n" - #1) in
         let, ("p", "r") := list_remove_nth_unsafe "l" "ip" in
         let, ("le", "gt") := partition "r" "p" in
         let, ("les", "gts") := ("qs" "le", "qs" "gt") in
-        list_append "les" (list_cons "p" "gts").
+        list_append "les" (list_cons "p"  "gts").
 
-
-  Lemma wp_remove_nth_unsafe {A} [_ : Inject A val] E (l : list A) (lv : val) (i : nat) :
-    {{{ ⌜ is_list l lv /\ i < length l ⌝ }}}
-      list_remove_nth_unsafe lv #i @ E
-    {{{ v, RET v;
-        ∃ e lv' l1 l2,
-          ⌜ l = l1 ++ e :: l2 ∧
-          length l1 = i /\
-          v = ((inject e), lv')%V ∧
-          is_list (l1 ++ l2) lv' ⌝ }}}.
-  Proof.
-    iIntros (φ (llv & il)) "hφ".
-    rewrite /list_remove_nth_unsafe. wp_pures.
-    wp_apply wp_remove_nth => //.
-    iIntros (?(?&?&?&?&?&?&?&?)) ; subst. wp_pures.
-    iApply "hφ". iModIntro. iExists _,_,_,_. intuition eauto.
-  Qed.
 
   Lemma filter_split_perm {A} (l : list A) f :
     l ≡ₚ List.filter f l ++ List.filter (fun x=>negb (f x)) l.
@@ -63,10 +35,9 @@ Section quicksort.
     destruct (f a) => /= ; rewrite -?Permutation_middle -IHl //.
   Qed.
 
-  Lemma Partition (xs : list Z) l (e : Z) e' :
-    e' = Val #e ->
+  Lemma Partition (xs : list Z) l (e : Z) :
     {{{ ⌜is_list xs l⌝ }}}
-      partition l e'
+      partition l (Val #e)
     {{{ le gt, RET (le, gt);
         ∃ xsle xsgt : list Z,
           ⌜is_list xsle le ∧ is_list xsgt gt
@@ -75,7 +46,7 @@ Section quicksort.
                    ∧ ⌜ ∀ x, In x xsgt → (e < x)%Z ⌝
     }}}.
   Proof.
-    iIntros (-> φ Lxs) "hφ".
+    iIntros (φ Lxs) "hφ".
     rewrite /partition. subst.
     wp_pures.
     wp_bind (list_filter _ _).
@@ -137,30 +108,35 @@ Section quicksort.
     {{{ ⌜is_list xs l⌝ }}}
       qs l
     {{{ v, RET v; ∃ xs', ⌜ is_list xs' v ∧ xs' ≡ₚ xs ∧ sorted xs' ⌝ }}}.
-  Proof with wp_pures.
+  Proof.
     iLöb as "Hqs". iIntros (xs l φ hl) "hφ".
-    rewrite {2}/qs... rewrite -/qs.
+    unfold qs at 2. wp_pures. fold qs.
     wp_bind (list_length _). iApply (wp_list_length $! hl).
-    iIntros "!>" (n) "->"...
-    case_bool_decide as hn...
-    (* an empty or singleton list is already sorted. *)
+    iIntros "!>" (n) "->". wp_pures.
+    case_bool_decide as hn ; wp_pures.
+    (* A list of length ≤ 1 is already sorted. *)
     { iApply "hφ". iExists xs. iPureIntro. intuition auto.
-      destruct xs => //. 1: constructor. destruct xs => //. simpl in hn. lia. }
+      destruct xs as [|x xs]; [|destruct xs as [|y zs]].
+      - constructor.            (* [] is sorted. *)
+      - do 2 constructor.       (* [x] is sorted. *)
+      - cbn in hn. lia.         (* If len xs ≤ 1 then xs can't be x::y::zs. *)
+    }
     (* pick a pivot index at random *)
-    wp_apply wp_rand => //. iIntros (ip) "_"...
+    wp_apply wp_rand. 1: auto. iIntros (ip) "_". wp_pures.
     (* pop the pivot from xs *)
     wp_apply (wp_remove_nth_unsafe _ xs l ip).
     { iPureIntro. split => //. apply (Nat.lt_le_trans _ _ _ (fin_to_nat_lt ip)).
       destruct xs => /= ; simpl in hn ; lia. }
     iIntros (pr_opt (p & r & pre & post & hpart & hpos & hpr & hr)).
-    rewrite hpr. repeat (wp_pure ; unfold partition ; progress fold partition).
+    rewrite hpr.
+    repeat (wp_pure ; unfold partition ; progress fold partition).
     (* partition xs \ p into smaller and larger elements *)
     wp_apply Partition => //.
-    iIntros (le gt (xsle & xsgt & (hle & hgt & hperm) & ple & pgt))...
+    iIntros (le gt (xsle & xsgt & (hle & hgt & hperm) & ple & pgt)). wp_pures.
     (* sort xs_gt *)
     wp_apply "Hqs" => //. iIntros (gts (xs_gt_s & Lgts & Pgts & Sgts)).
     (* sort xs_le *)
-    wp_apply "Hqs" => //. iIntros (les (xs_le_s & Lles & Ples & Sles))...
+    wp_apply "Hqs" => //. iIntros (les (xs_le_s & Lles & Ples & Sles)). wp_pures.
     (* re-assemble the sorted results *)
     replace (#p) with (inject p) by auto.
     wp_apply wp_list_cons => //. iIntros (p_xs_gt_s h_p_xs_gt).
