theories/eris/tutorial/tutorial.v
@@ -1,2 +1,6 @@
 From clutch.eris.tutorial Require Import
-  basic bloom_filter_single bloom_filter_multi hash_interface.
+  basic
+  bloom_filter_single bloom_filter_multi
+  hash_interface
+  quicksort
+.
